Save

src/Monad.v
@@ -1,8 +1,11 @@
+From iris.algebra Require Import gmap.
 Require Import FunctionalExtensionality.
 From stdpp Require Import binders strings.
 From iris.proofmode Require Import tactics.
 From iris.base_logic.lib Require Import wsat.
 From iris.base_logic.lib Require Import gen_heap.
+From iris.program_logic Require Export  adequacy.
+
 Require Import Ctypes.
 
 Module monad.
@@ -14,6 +17,10 @@ Module monad.
     Context ( bind : forall X Y, M X -> (X -> M Y) -> M Y ).
     Arguments ret {_} x.
     Arguments bind {_ _} x f.
+    Inductive err (X: Type) : Type :=
+    | Erro : Errors.errmsg -> err X
+    | Res : X -> err X.
+
     Class MonadProp :=
       {
         left_id (X Y : Type) (a : X) (f : X -> M Y) : bind (ret a) f = f a;
@@ -30,39 +37,43 @@ Module monad.
         state : Type;
         ret : forall (X : Type), X -> M X;
         bind : forall X Y, M X -> (X -> M Y) -> M Y;
-        (* run : forall X, M X -> state -> state * X; *)
+        run : forall X, M X -> state -> err (state * X);
         prop : MonadProp M ret bind
       }.
   
 End monad.
 
-Module weakestpre.
-  Export monad.
+(* Module weakestpre. *)
+(*   Export monad. *)
 
-  Class Mwp {X} (Λ : monad) (PROP : Type) :=
-    mwp : ((M Λ) X) → (X → PROP) → PROP.
-  Instance: Params (@Mwp) 7 := {}.
 
-  Notation "'WP' e |{ Φ } |" := (mwp e Φ)
-                                      (at level 20, e, Φ at level 200, only parsing) : bi_scope.
-  Notation "'WP' e |{ v , Q } |" := (mwp e (λ v, Q))
-  (at level 20, e, Q at level 200,
-   format "'[' 'WP'  e  '[ ' |{  v ,  Q  } | ']' ']'") : bi_scope.
+(*   Class Mwp {X} (Λ : monad) (PROP : Type) := *)
+(*     mwp : ((M Λ) X) → (X → PROP) → PROP. *)
+(*   Instance: Params (@Mwp) 7 := {}. *)
 
-  Notation "'|{{' P } } | e |{{ x .. y , 'RET' pat ; Q } } |" :=
-    ( □ ∀ Φ,
-       P -∗ (∀ x, .. (∀ y, Q -∗ Φ pat) .. ) -∗ WP e |{ Φ }|)%I
-         (at level 20, x closed binder, y closed binder,
-          format "'[hv' |{{  P  } } |  '/  ' e  '/'  |{{  x  ..  y ,  RET  pat ;  Q  } } | ']'") : bi_scope.
+(*   Notation "'WP' e |{ Φ } |" := (mwp e Φ) *)
+(*                                       (at level 20, e, Φ at level 200, only parsing) : bi_scope. *)
+(*   Notation "'WP' e |{ v , Q } |" := (mwp e (λ v, Q)) *)
+(*   (at level 20, e, Q at level 200, *)
+(*    format "'[' 'WP'  e  '[ ' |{  v ,  Q  } | ']' ']'") : bi_scope. *)
 
-End weakestpre.
+(*   Notation "'|{{' P } } | e |{{ x .. y , 'RET' pat ; Q } } |" := *)
+(*     ( □ ∀ Φ, *)
+(*        P -∗ (∀ x, .. (∀ y, Q -∗ Φ pat) .. ) -∗ WP e |{ Φ }|)%I *)
+(*          (at level 20, x closed binder, y closed binder, *)
+(*           format "'[hv' |{{  P  } } |  '/  ' e  '/'  |{{  x  ..  y ,  RET  pat ;  Q  } } | ']'") : bi_scope. *)
+
+(* End weakestpre. *)
 
 Module gensym.
   Import monad.
-  Open Scope positive_scope.
+  Local Open Scope positive_scope.
   
   Definition ident := positive.
   Definition state := gmap ident type.
+  Definition empty_state : state := gmap_empty.
+  Definition state_to_list (s : state) := gmap_to_list s.
+  
   (* %%%%%%%%%%%%%%%%%%%%%%%%%%%%%%%%%%%%%%%%%%%%%%%%%%%%%%%%%ùùùùù*)
   Inductive sig (X : Type) : Type :=
   | Err : Errors.errmsg -> sig X
@@ -107,26 +118,8 @@ Module gensym.
 
   Voila, l'idée
    *)
-
-  Inductive err (X: Type) : Type :=
-  | Erro : Errors.errmsg -> err X
-  | Res : X -> err X.
-
-  Arguments Erro [X].
-  Arguments Res [X].
-
-  Definition fresh (s : state) := map_fold (fun x _ res => Pos.max res (x+1)) 1 s.
   
-  Fixpoint run {X} (m : mon X) : state -> state * err X :=
-    match m with
-    | ret v => fun s => (s, Res v)
-    | op (Err e) => fun s => (s, Erro e)
-    | op (Gensym t f) =>
-        fun s =>
-          let l := fresh s in
-          run (f l) ({[l := t]} ∪ s)
-    end.
-  
+
   Lemma lid : forall X Y (a : X) (f : X -> mon Y), bind (ret a) f = f a.
   Proof. auto. Qed.
 
@@ -156,117 +149,621 @@ Module gensym.
   Instance mP : @MonadProp mon (@ret) (@bind).
   Proof. split; eauto. Qed.
 
-  Canonical Structure gensym_monad := @Monad mon (gmap ident type) (@ret) (@bind) mP.
+  Arguments Erro [X].
+  Arguments Res [X].
+  Open Scope positive_scope.
+
+  Definition fresh (s : state) :=
+    map_fold (fun x _ res => Pos.max res (x+1)) 1 s.
+  
+  Fixpoint run {X} (m : mon X) : state -> err (state * X) :=
+    match m with
+    | ret v => fun s => Res (s, v)
+    | op (Err e) => fun s => Erro e
+    | op (Gensym t f) =>
+      fun s =>
+        let l := fresh s in
+        run (f l) (<[l := t]>s)
+    end.
+  
+
+  Canonical Structure gensym_monad := @Monad mon state (@ret) (@bind) (@run) mP.
+
 End gensym.
 
 Module weakestpre_gensym.
-  Export weakestpre.
+  Import monad.
   Export gensym.
   Export gen_heap.
-   
-  Class irisG (Σ : gFunctors) :=
-    IrisG {
-        iris_invG :> invG.invG Σ;
-        state_interp : state → iProp Σ;
-      }.
-  Global Opaque iris_invG.
-  
-  Class heapG Σ :=
-    HeapG {
-        heapG_invG : invG.invG Σ;
-        heapG_gen_heapG :> gen_heapG positive type Σ;
-      }.
-  
-  Instance heapG_irisG `{!heapG Σ} : irisG Σ := {
-                                                 iris_invG := heapG_invG;
-                                                 state_interp σ := gen_heap_ctx σ%I;
-                                               }.
-
   (** Override the notations so that scopes and coercions work out *)
   Notation "l ↦ t" :=
     (mapsto (L:=ident) (V:=type) l 1 t) (at level 20) : bi_scope.
 
   Notation "\s l" :=
     (∃ t, l ↦ t)%I (at level 20) : bi_scope.
+
+  Notation "P ⨈ Q" := (((P -∗ False) ∗ (Q -∗ False)) -∗ False)%I (at level 19) : bi_scope.
+  
+  Class heapG Σ :=
+    HeapG {
+        heapG_gen_heapG :> gen_heapG ident type Σ;
+      }.
+  
+  Class irisG (Σ : gFunctors) :=
+    IrisG {
+        state_interp : state → iProp Σ;
+      }.
+  Global Opaque iris_invG.
+  
+  Instance heapG_irisG `{!heapG Σ} : irisG Σ := {
+                                                 state_interp σ := gen_heap_ctx σ%I;
+                                               }.
   
   Section mwp.
-    Context {X : Type} `{!heapG Σ}.
-    Implicit Types P : iProp Σ.
-    Implicit Types Φ : X → iProp Σ.
-    Implicit Types v : X.
-    Implicit Types e : mon X.
-    
-    Fixpoint mwp `{!irisG Σ} (e1 : mon X) (Q : X -> iProp Σ) : iProp Σ :=
+    Context `{!heapG Σ}.
+    Fixpoint mwp {X} (e1 : mon X) (Q : X -> iProp Σ) : iProp Σ :=
       match e1 with
       | ret v => Q v
-      | op (Err e) => False
+      | op (Err e) => True
       | op (Gensym t f) =>
         ∀ l, l ↦ t -∗ mwp (f l) Q
-      end%I.
-
-    Global Instance mwp' `{!irisG Σ} : @Mwp X gensym_monad (iProp Σ) := mwp.
-    
-    Global Instance mwp_ne e n :
-      Proper (pointwise_relation _ (dist n) ==> dist n) (mwp e).
-    Proof.
-      revert e. induction (lt_wf n) as [n _ IH]=> e P P' HP.
-      revert e. fix e 1.
-      destruct e0.
-      * apply HP.
-      * destruct s.
-        ** simpl. auto.
-        ** simpl. do 3 f_equiv. apply e. 
-    Qed.
-
-    Global Instance mwp_proper e :
-      Proper (pointwise_relation _ (≡) ==> (≡)) (mwp e).
-    Proof.
-        by intros Φ Φ' ?; apply equiv_dist=>n; apply mwp_ne=>v; apply equiv_dist.
-    Qed.
-
-    Lemma mwp_unfold e Φ :
-      WP e |{ Φ }| ⊣⊢ mwp e Φ.
-    Proof. auto. Qed.
-
-    Lemma mwp_value' Φ v : Φ v ⊢ WP ret v |{ Φ }|.
-    Proof. eauto. Qed.
-    Lemma mwp_value_inv' Φ v : WP ret v |{ Φ }| -∗ Φ v.
-    Proof. eauto. Qed.
-  
-    Lemma mwp_mono e Φ Ψ :
-      WP e |{ Φ }| -∗ (∀ v, Φ v -∗ Ψ v) -∗ WP e |{ Ψ }|.
-    Proof.
-      iIntros "HA HB". rewrite !mwp_unfold. revert e. fix e 1.
-      destruct e0.
-      { iApply "HB". iApply "HA". }
-      { destruct s.
-        { simpl. auto. }
-        { simpl. iIntros (l) "HC". iDestruct ("HA" with "HC") as "HA".
-          iPoseProof "HB" as "HB". apply e. }}
-    Qed.
-      
-    Lemma mwp_bind e f Φ Φ' :
-      WP e |{ Φ' }| -∗ (∀ v,  Φ' v -∗ WP (f v) |{ Φ }|) -∗ WP bind e f |{ Φ }|%I.
-    Proof.
-      iIntros "HA HB". rewrite !mwp_unfold. revert e. fix e 1.
-      destruct e0.
-      { iApply "HB". iApply "HA". }
-      { destruct s.
-        { simpl. auto. }
-        { simpl. iIntros (l) "HC". iDestruct ("HA" with "HC") as "HA".
-          iPoseProof "HB" as "HB". apply e. }}
-    Qed.
-
-    Lemma mwp_frame_l e Φ R : R ∗ WP e |{ Φ }| ⊢ WP e |{ v, R ∗ Φ v }|.
-    Proof. iIntros "[? H]". iApply (mwp_mono with "H"); auto with iFrame. Qed.
-    Lemma mwp_frame_r e Φ R : WP e |{ Φ }| ∗ R ⊢ WP e |{ v, Φ v ∗ R }|.
-    Proof. iIntros "[H ?]". iApply (mwp_mono with "H"); auto with iFrame. Qed.
-
+      end%I.    
   End mwp.
+
+  Notation "'WP' e |{ Φ } |" := (mwp e Φ)
+                                  (at level 20, e, Φ at level 200, only parsing) : bi_scope.
   
+  Notation "'WP' e |{ v , Q } |" := (mwp e (λ v, Q))
+                                      (at level 20, e, Q at level 200,
+                                       format "'[' 'WP'  e  '[ ' |{  v ,  Q  } | ']' ']'") : bi_scope.
+  
+  Notation "'|{{' P } } | e |{{ x .. y , 'RET' pat ; Q } } |" :=
+    ( ∀ Φ,
+        P -∗ (∀ x, .. (∀ y, Q -∗ Φ pat) .. ) -∗ WP e |{ Φ }|)%I
+                                                             (at level 20, x closed binder, y closed binder,
+                                                              format "'[hv' |{{  P  } } |  '/  ' e  '/'  |{{  x  ..  y ,  RET  pat ;  Q  } } | ']'") : bi_scope.
+
+    
+    Class heapPreG Σ :=
+      HeapPreG {
+          heap_preG_heap :> gen_heapPreG ident type Σ
+        }.
+
+    Definition heapΣ : gFunctors := #[gen_heapΣ ident type].
+    Instance subG_heapPreG {Σ} : subG heapΣ Σ → heapPreG Σ.
+    Proof. solve_inG. Qed.
+
+    Definition adequate `{heapG Σ} {X} (e : mon X) (σ1 : state) (φ : X → state → iProp Σ) :=
+      (match run e σ1 with
+       | Res (σ2,v) => φ v σ2
+       | Erro e => True
+      end)%I.
+
+    
+    
+    Open Scope bi_scope.
+
+    Lemma adequate_step {X} `{heapG Σ} σ φ t m :
+      adequate (op (Gensym t m)) σ (λ (v : X) (_ : state), φ v) ∗-∗
+               adequate (m (fresh σ)) (<[ fresh σ := t ]>σ) (λ (v : X) (_ : state), φ v).
+    Proof. iSplit; eauto. Qed.
+
+    Print gmap.alloc_updateP'.
+
+    Lemma disjointeness_fresh `{heapG Σ} : forall (σ : gmap ident type), σ !! (fresh σ) = None.
+    Proof.
+      epose fupd_mask_weaken.
+    Admitted.
+
+    (* Lemma soundness `{!heapPreG heapΣ} {X} P Q : forall (e : mon X) σ, *)
+    (*   (state_interp σ -∗ *)
+    (*   |{{ P }}| e |{{ v, RET v; Q v }}|) -> *)
+    (*   adequate e σ (fun v _ => Q v). *)
+    (* Proof. *)
+    (*   fix e 1. *)
+    (*   destruct e0; simpl; intros. *)
+    (*   * unfold adequate. simpl. *)
+    (*     iMod (gen_heap_init σ) as (?) "Hh". *)
+    
+    (* Lemma gen_heap_alloc σ l v : *)
+    (*   σ !! l = None → *)
+    (*   gen_heap_ctx σ -∗ gen_heap_ctx (<[l:=v]>σ) ∗ l ↦ v ∗ meta_token l ⊤. *)
+    (* Proof. *)
+    (*   iIntros (P) "HA". *)
+    (*   rewrite /gen_heap_ctx mapsto_eq /mapsto_def meta_token_eq /meta_token_def /=. *)
+    (*   iDestruct "HA" as  (m) "HA". *)
+    (*   iDestruct "HA" as "[HA [HB HC]]". *)
+    (*   iSplitL "HA HB". *)
+    (*   * iExists (<[l:=v]>m). *)
+    (*     rewrite to_gen_heap_insert. *)
+    (*     iSplit. *)
+    (*     ** *)
+    (*       epose (not_elem_of_dom (D:=gset ident)). *)
+    (*       admit. *)
+    (*     **  *)
+
+    Lemma wp_adequacy {X} `{heapG Σ} (e : mon X) σ (φ : X -> iProp Σ) :
+      ((|==> state_interp σ ∗ WP e |{ v, φ v }|) ->
+                                          |==> adequate e σ (λ v _, φ v) )%I.
+    Proof.
+      revert e σ. fix e 1.
+      destruct e0.
+      iStartProof.
+      - iIntros (x0 HA).
+        iPoseProof HA as "HA". iMod "HA" as "HA". iDestruct "HA" as "[HA HB]". iApply "HB".
+      - iIntros (σ HA).
+        destruct s.
+        + unfold adequate. simpl. iStartProof. trivial.
+        + iApply adequate_step. iApply e.
+          iPoseProof HA as "HA".
+          iMod "HA" as "HA".
+          iDestruct "HA" as "[HA HB]".
+          simpl. pose disjointeness_fresh. apply (gen_heap_alloc σ _ t)  in e0.
+          iPoseProof e0 as "HC".
+          iDestruct ("HC" with "HA") as "HE".
+          iMod "HE" as "HE".
+          iModIntro.
+          iDestruct "HE" as "[HA [HD HE]]".
+          iFrame. iApply "HB". iFrame.
+    Qed.
+
+    Import uPred.    
+
+    Lemma test `{!heapG Σ} t t' : forall σ l,
+        σ !! l = None ->
+            state_interp σ -∗  state_interp (<[l:=t]> σ) ∗ l ↦ t'.
+    Proof.
+      iIntros (σ l P) "HA". unfold state_interp. simpl.
+      rewrite /gen_heap_ctx mapsto_eq /mapsto_def.
+      epose own_valid_2.
+      epose gen_heap_singleton_included.
+      epose auth.auth_both_valid.
+      epose to_gen_heap_insert.
+      epose sep_assoc'.
+      iSplitL. 
+      - iExists m.
+        + iSplitL "HA".
+          * iDestruct "HA" as "%". iPureIntro. apply dom_insert_subseteq_compat_l. apply H.
+          * iSplitL "HB".
+            -- 
+                
+      
+    Lemma next_step `{!heapG Σ} {X} P Q t : forall m σ,
+    state_interp σ ∗ |{{ P }}| op (Gensym t m)  |{{ (v : X), RET v; Q v }}|
+    ∗-∗  state_interp (<[fresh σ:=t]> σ) ∗ |{{ P }}| m (fresh σ)  |{{ (v : X), RET v; Q v }}|.
+    Proof.
+      iIntros (m σ).
+      iSplit.
+      * iIntros "HA". iDestruct "HA" as "[HA HB]".
+
+        
+                         
+        
+
+    
+    Lemma soundness `{!heapG Σ} {X} P Q (e : mon X) σ:
+      (state_interp σ ∗
+      |{{ P }}| e |{{ v, RET v; Q v }}|) ->
+      match run e σ with
+      | Erro _ => True
+      | Res (σ',x) => P -> Q x
+      end.
+    Proof.
+      revert e σ. fix e 1.
+      destruct e0; intros.
+      - intro. iPoseProof H as "HA". iDestruct "HA" as "[HA HB]".
+        iApply "HB".        
+        + iApply H0.
+        + eauto.
+      - destruct s.
+        + simpl. trivial.
+        + simpl. apply e.
+
+          
+
+
+          epose (gen_heap_init σ).
+      
+    
+    Section mwp.
+      Context `{!heapG heapΣ}.
+      Fixpoint mwp {X} (e1 : mon X) (Q : X -> iProp heapΣ) : iProp heapΣ :=
+        match e1 with
+        | ret v => Q v
+        | op (Err e) => True
+        | op (Gensym t f) =>
+          ∀ l, l ↦ t -∗ mwp (f l) Q
+        end%I.
+
+    End mwp.
+
+    Notation "'WP' e |{ Φ } |" := (mwp e Φ)
+                                    (at level 20, e, Φ at level 200, only parsing) : bi_scope.
+
+    Notation "'WP' e |{ v , Q } |" := (mwp e (λ v, Q))
+                                        (at level 20, e, Q at level 200,
+                                         format "'[' 'WP'  e  '[ ' |{  v ,  Q  } | ']' ']'") : bi_scope.
+
+    Notation "'|{{' P } } | e |{{ x .. y , 'RET' pat ; Q } } |" :=
+      ( ∀ Φ,
+          P -∗ (∀ x, .. (∀ y, Q -∗ Φ pat) .. ) -∗ WP e |{ Φ }|)%I
+                                                               (at level 20, x closed binder, y closed binder,
+                                                                format "'[hv' |{{  P  } } |  '/  ' e  '/'  |{{  x  ..  y ,  RET  pat ;  Q  } } | ']'") : bi_scope.
+    Open Scope bi_scope.
+    Print ucmraT. Print iResUR. Print gFunctors. Print fin. Locate Fin. Print Fin.
+    Lemma test `{!heapG heapΣ} {X} P Q (e : mon X) :
+      (state_interp empty_state -∗ |{{ P }}| e |{{ v, RET v; Q v }}|) ->
+    |{{ P }}| e |{{ v, RET v; Q v }}|.
+    Proof. Print heapG. Locate heapG.
+    Admitted.
+
+    Lemma soundness `{!heapG heapΣ} {X} P Q (e : mon X) σ:
+      (state_interp σ -∗
+      |{{ P }}| e |{{ v, RET v; Q v }}|) ->
+      match run e σ with
+      | Erro _ => True
+      | Res (σ',x) => P -> Q x
+      end.
+    Proof.
+      revert e σ. fix e 1. destruct e0.
+      - intros. simpl. intro. iApply H.
+        + unfold gen_heap_ctx. iExists empty. iSplit.
+          * iPureIntro. Print subseteq_dom.
+            epose (@subseteq_dom _ _ (gset ident) _ _ _ _ _ _ _ _ _ _ _ _ _ _ _ _ _ ∅ σ).
+            apply s.
+            apply map_subseteq_spec.
+            intros. erewrite lookup_empty in H1. inversion H1.
+          *  admit.
+        + iApply H0.
+        + iIntros (v) "HA".
+          iApply "HA".
+      - intros. simpl. destruct s; eauto.
+        apply e. iIntros "HA".
+        iIntros. Print erased_step.
+
+
+
+
+        Section mwp_proof.
+          Context `{!heapG Σ}.
+          Lemma mwp_value' {X} Φ (v : X) : Φ v ⊢ WP ret v |{ Φ }|.
+          Proof. auto. Qed.
+          Lemma mwp_value_inv' {X} Φ (v : X) : WP ret v |{ Φ }| -∗ Φ v.
+          Proof. auto. Qed.
+
+          Lemma mwp_mono {X} e Φ Ψ :
+            WP e |{ Φ }| -∗ (∀ (v : X), Φ v -∗ Ψ v) -∗ WP e |{ Ψ }|.
+          Proof.
+            iIntros "HA HB". revert e. fix e 1.
+            destruct e0.
+            { iApply "HB". iApply "HA". }
+            { destruct s.
+              { simpl. trivial. }
+              { simpl. iIntros (l) "HC". iDestruct ("HA" with "HC") as "HA".
+                iPoseProof "HB" as "HB". apply e. }}
+          Qed.
+
+          Lemma mwp_bind {X Y} (e : mon X) (f :  X → mon Y) (Φ : Y -> iProp Σ)  (Φ' : X -> iProp Σ) :
+            WP e |{ Φ' }| -∗ (∀ v,  Φ' v -∗ WP (f v) |{ Φ }|) -∗ WP bind e f |{ Φ }|%I.
+          Proof.
+            iIntros "HA HB". revert e. fix e 1.
+            destruct e0.
+            { iApply "HB". iApply "HA". }
+            { destruct s.
+              { simpl. auto. }
+              { simpl. iIntros (l) "HC". iDestruct ("HA" with "HC") as "HA".
+                iPoseProof "HB" as "HB". apply e. }}
+          Qed.
+
+          Open Scope bi_scope.
+          Lemma mwp_gensym t : WP gensym t |{ l, l ↦ t }|.
+          Proof. simpl. iIntros. iFrame. Qed.
+
+          Lemma mwp_frame_l {X} (e : mon X) Φ R : R ∗ WP e |{ Φ }| ⊢ WP e |{ v, R ∗ Φ v }|.
+          Proof. iIntros "[? H]". iApply (mwp_mono with "H"). auto with iFrame. Qed.
+          Lemma mwp_frame_r {X} (e : mon X) Φ R : WP e |{ Φ }| ∗ R ⊢ WP e |{ v, Φ v ∗ R }|.
+          Proof. iIntros "[H ?]". iApply (mwp_mono with "H"); auto with iFrame. Qed.
+
+
+
+        End mwp_proof.
+
+        Open Scope bi_scope.
+
+
+        Lemma soundness `{!heapG Σ} {X} P Q (e : mon X) :
+        |{{ P }}| e |{{ v, RET v; Q v }}| ->
+                                          (forall n (s : state), P n s -> Q (run e s)).
+
+
 End weakestpre_gensym.
 
+From iris.proofmode Require Import coq_tactics reduction.
+From iris.proofmode Require Export tactics.
 
+Module proofmode.
+  Export weakestpre_gensym.
+  Open Scope bi_scope.
+  Ltac early S := iIntros (Φ) S.
+  Section proofmode_intro.
+    Context `{!heapG Σ}.    
+    
+    Lemma gensym_spec t :
+    |{{ True }}| gensym t |{{ l, RET l; l ↦ t }}|.
+    Proof. iIntros (l) "HA HB". iApply "HB". Qed.
+    
+    Lemma ret_spec {X} (v : X) :
+    |{{ True }}| ret v |{{ v', RET v'; ⌜ v' = v ⌝  }}|.
+    Proof. early "HA HB". iApply "HB". auto. Qed.
+    
+    Lemma ret_spec_bis {X} (v : X) (Q : X -> iProp Σ) :
+      Q v
+      <->
+    |{{ True }}| ret v |{{ v', RET v'; Q v' }}|.
+    Proof.
+      split.
+      - intro. early "HA HB". iApply "HB". iApply H.
+      - intro. iApply H; eauto.
+    Qed. 
+    
+    Lemma error_spec {X} (Q : X -> iProp Σ) e :
+    |{{ True }}| error e |{{ v, RET v; Q v }}|.
+    Proof. early "HA HB". iApply "HA". Qed.
+    
+    Lemma bind_spec {X Y} (e : mon X) (f : X -> mon Y) Φ' Φ'' H :
+    |{{ H }}| e |{{ v, RET v; Φ'' v }}| ->
+                                        (∀ v, |{{ Φ'' v }}| (f v) |{{ v', RET v'; Φ' v' }}|) ->
+    |{{ H }}| (bind e f) |{{ v, RET v; Φ' v}}|.
+    Proof.
+      intros. early "HA HB".
+      iApply (mwp_bind e f _ Φ'' with "[HA]").
+      - iApply (H0 with "[HA]"); auto. 
+      - iIntros (v) "HC". iApply (H1 with "[HC]"); auto.
+    Qed.
+    
+    Lemma frame_r {X} H R Φ' (e : mon X) :
+    |{{ H }}| e |{{ v, RET v; Φ' v }}| ->
+    |{{ H ∗ R }}| e |{{ v, RET v; Φ' v ∗ R }}|.
+    Proof.
+      intro P. early "HA HB". iDestruct "HA" as "[HA HC]".
+      iApply (P with "[HA]"); auto.
+      iIntros (v) "HA". iApply "HB". iFrame.
+    Qed.
+
+    Lemma frame_l {X} H R Φ' (e : mon X) :
+    |{{ H }}| e |{{ v, RET v; Φ' v }}| ->
+    |{{ R ∗ H }}| e |{{ v, RET v; R ∗ Φ' v }}|.
+    Proof. intro P. early "HA HB". iDestruct "HA" as "[HA HC]".
+           iApply (P with "[HC]"); auto.
+           iIntros (v) "HC". iApply "HB". iFrame.
+    Qed.
+
+    Lemma consequence_post {X} Φ'' H Φ'  (e : mon X) :
+      (forall v, Φ'' v -∗ Φ' v) ->
+    |{{ H }}| e |{{ v, RET v; Φ'' v }}| ->
+    |{{ H }}| e |{{ v, RET v; Φ' v }}|.
+    Proof.
+      intros P P'. early "HA HB".
+      iApply (P' with "[HA]"); auto.
+      iIntros (v) "HA". iApply "HB". iApply P. iApply "HA".
+    Qed.
+
+    Lemma consequence_pre {X} H' Φ' (H : iProp Σ)  (e : mon X) :
+      (H -∗ H') ->
+    |{{ H' }}| e |{{ v, RET v; Φ' v }}| ->
+    |{{ H }}| e |{{ v, RET v; Φ' v }}|.
+    Proof.
+      intros P P'. early "HA HB".
+      iApply (P' with "[HA]"); auto.
+      iApply P. iApply "HA".
+    Qed.
+    
+    Lemma tLeft {X} (Q : X -> iProp Σ) (R : X -> iProp Σ) S (e : mon X) :
+    |{{ S }}| e |{{ v, RET v; R v }}| ->
+    |{{ S }}| e |{{ v, RET v; R v ⨈ Q v }}|.
+    Proof.
+      intro H. early "HA HB".
+      iApply (H with "[HA]"); auto.
+      iIntros (v) "HA". iApply "HB". iIntros "HB". iDestruct "HB" as "[HB HC]".
+      iApply "HB". iApply "HA".
+    Qed.
+
+    Lemma tRight {X} (Q : X -> iProp Σ) (R : X -> iProp Σ) S (e : mon X) :
+    |{{ S }}| e |{{ v, RET v; Q v }}| ->
+    |{{ S }}| e |{{ v, RET v; R v ⨈ Q v }}|.
+    Proof.
+      intro H. early "HA HB".
+      iApply (H with "[HA]"); auto.
+      iIntros (v) "HA". iApply "HB". iIntros "HB". iDestruct "HB" as "[HB HC]".
+      iApply "HC". iApply "HA".
+    Qed.
+
+    Lemma ret_spec_complete {X} (Q : X -> iProp Σ) S (v : X) :
+      (S -∗ Q v) ->
+    |{{ S }}| ret v |{{ v', RET v'; Q v' }}|.
+    Proof.
+      intro. early "HA HB". iApply "HB". iDestruct (H with "HA") as "HA". iApply "HA".
+    Qed.
+
+    
+    Lemma True_pre_l {X} H Φ' (e : mon X) :
+    |{{ True ∗ H}}| e |{{ v, RET v; Φ' v }}| ->
+    |{{ H }}| e |{{ v, RET v; Φ' v }}|.
+    Proof.
+      intro P. early "HA HB". 
+      iApply (P with "[HA]"); auto.
+    Qed.
+
+    Lemma True_pre_r {X} H Φ' (e : mon X) :
+    |{{ H ∗ True}}| e |{{ v, RET v; Φ' v }}| ->
+    |{{ H }}| e |{{ v, RET v; Φ' v }}|.
+    Proof.
+      intro P. early "HA HB". 
+      iApply (P with "[HA]"); auto.
+    Qed.
+
+  End proofmode_intro.
+
+  Ltac tFrame_l := apply True_pre_r; apply frame_l; eauto.
+  Ltac tFrame_r := apply True_pre_l; apply frame_r; eauto.
+  
+  Section proofmode_divers.
+    Context `{!heapG Σ}.
+    
+    Lemma comm_post {X} R Φ' (e : mon X) H :
+    |{{ H }}| e |{{ v, RET v; Φ' v ∗ R v }}| ->
+    |{{ H }}| e |{{ v, RET v; R v ∗ Φ' v}}|.
+    Proof.
+      intro P. early "HA HB".
+      iApply (P with "[HA]"); auto.
+      iIntros (v) "HA". iApply "HB". iDestruct "HA" as "[HA HC]". iFrame.
+    Qed.
+
+    Lemma comm_pre {X} R Φ' (e : mon X) H :
+    |{{ R ∗ H}}| e |{{ v, RET v; Φ' v }}| ->
+    |{{ H ∗ R}}| e |{{ v, RET v; Φ' v}}|.
+    Proof.
+      intro P. early "HA HB".
+      iApply (P with "[HA]"); auto.
+      iDestruct "HA" as "[HA HC]". iFrame.
+    Qed.
+
+    Lemma impl_post_id {X} R P Φ' (e : mon X) :
+    |{{ R }}| e |{{ v, RET v; Φ' v }}| ->
+    |{{ R }}| e |{{ v, RET v; P -∗ P ∗ Φ' v}}|.
+    Proof.
+      intro H. early "HA HB".
+      iApply (H with "[HA]"); auto.
+      iIntros (v) "HA". iApply "HB". iIntros "HB". iFrame.
+    Qed.
+
+    Lemma impl_post {X} R P Φ' (e : mon X) :
+    |{{ R }}| e |{{ v, RET v; Φ' v }}| ->
+    |{{ R }}| e |{{ v, RET v; P -∗ Φ' v}}|.
+    Proof.
+      intro H. early "HA HB".
+      iApply (H with "[HA]"); auto.
+      iIntros (v) "HA". iApply "HB". eauto.
+    Qed.
+
+    Lemma star_assoc_post {X} R Q S T (e : mon X) :
+    |{{ T }}| e |{{ v, RET v; R v ∗ (Q v ∗ S v)}}| <->
+    |{{ T }}| e |{{ v, RET v; (R v ∗ Q v) ∗ S v }}|.
+    Proof.
+      split; intro H; early "HA HB";
+        iApply (H with "[HA]"); try (iApply "HA");
+          iIntros (v) "HA"; iApply "HB".
+      - iDestruct "HA" as "[HA [HB HC]]". iFrame.
+      - iDestruct "HA" as "[[HA HB] HC]". iFrame.
+    Qed.
+
+    Lemma star_assoc_pre {X} R Q S T (e : mon X) :
+    |{{ (T ∗ R) ∗ S }}| e |{{ v, RET v; Q v }}| <->
+    |{{ T ∗ (R ∗ S) }}| e |{{ v, RET v; Q v }}|.
+    Proof.
+      split; intro H; early "HA HB"; iApply (H with "[HA]"); eauto.
+      - iDestruct "HA" as "[HA [HB HC]]". iFrame.
+      - iDestruct "HA" as "[[HA HB] HC]". iFrame.
+    Qed.
+
+    Lemma impl_true_pre {X} (R : X -> iProp Σ) Q (e : mon X) :
+    |{{ Q }}| e |{{ v', RET v'; R v'}}| ->
+    |{{ True -∗ Q }}| e |{{ v', RET v'; R v'}}|.
+    Proof.
+      intro H. early "HA HB". iApply (H with "[HA]"); eauto. iApply "HA"; auto.
+    Qed.
+
+    Lemma impl_true_post {X} (R : X -> iProp Σ) Q (e : mon X) :
+    |{{ Q }}| e |{{ v', RET v'; R v'}}| ->
+    |{{ Q }}| e |{{ v', RET v'; True -∗ R v'}}|.
+    Proof.
+      intro H. early "HA HB". iApply (H with "[HA]"); eauto.
+      iIntros (v') "HA". iApply "HB". auto.
+    Qed.
+
+    Lemma exist {X Y} v (R : Y -> X -> iProp Σ) Q (e : mon X) :
+    |{{ Q }}| e |{{ v', RET v'; R v v'}}| ->
+    |{{ Q }}| e |{{ v', RET v'; ∃ t, R t v'}}|.
+    Proof.
+      intro H. early "HA HB".
+      iApply (H with "[HA]"); auto.
+      iIntros (v0) "HC". iApply "HB". iExists v. iFrame.
+    Qed.
+
+    Lemma exists_frame_r {X Y} v (Q : Y -> iProp Σ) R (e : mon X) :
+    |{{ True }}| e |{{ v', RET v'; R v v' }}| ->
+    |{{ Q v }}| e |{{ v', RET v'; ∃ t, R t v' ∗ Q t}}|.
+    Proof.
+      intro.
+      iApply (exist v). tFrame_r.
+    Qed.
+
+    Lemma exists_frame_l {X Y} v (Q : Y -> iProp Σ) R (e : mon X) :
+    |{{ True }}| e |{{ v', RET v'; R v v'}}| ->
+    |{{ Q v }}| e |{{ v', RET v'; ∃ t, Q t ∗ R t v'}}|.
+    Proof.
+      intro.
+      iApply (exist v).
+      tFrame_l.
+    Qed.
+
+    Lemma exists_out_l {X Y} (Q : iProp Σ) (R : Y -> X -> iProp Σ) S (e : mon X) :
+    |{{ S }}| e |{{ v', RET v'; Q ∗ ∃ t, R t v' }}| ->
+    |{{ S }}| e |{{ v', RET v'; ∃ t, Q ∗ R t v'}}|.
+    Proof.
+      intro H. early "HA HB".
+      iApply (H with "[HA]"); auto.
+      iIntros (v) "HA". iApply "HB". iDestruct "HA" as "[HA HB]". iDestruct "HB" as (t) "HB".
+      iExists t. iFrame.
+    Qed.
+
+    Lemma exists_out_r {X Y} (Q : iProp Σ) (R : Y -> X -> iProp Σ) S (e : mon X) :
+    |{{ S }}| e |{{ v', RET v'; (∃ t, R t v') ∗ Q }}| ->
+    |{{ S }}| e |{{ v', RET v'; ∃ t, R t v' ∗ Q }}|.
+    Proof.
+      intro H. early "HA HB".
+      iApply (H with "[HA]"); auto.
+      iIntros (v) "HA". iApply "HB". iDestruct "HA" as "[HA HB]". iDestruct "HA" as (t) "HA".
+      iExists t. iFrame.
+    Qed.
+
+    Lemma ret_frame_l {X Y} (R : Y -> iProp Σ) (R' Φ' : X -> iProp Σ) (v' : X) (v'': Y) : 
+      Φ' v' -> R v'' = R' v' ->
+    |{{ R v'' }}| ret v' |{{ v, RET v; R' v ∗ Φ' v }}|.
+    Proof.
+      intros H H'. early "HA HB".
+      iApply mwp_value'. iApply "HB". rewrite H'. iFrame. iApply H.
+    Qed.
+
+    Lemma ret_frame_r {X Y} (R : Y -> iProp Σ) (R' Φ' : X -> iProp Σ) (v' : X) (v'' : Y): 
+      Φ' v' -> R v'' = R' v' ->
+    |{{ R v'' }}| ret v' |{{ v, RET v; Φ' v ∗ R' v }}|.
+    Proof.
+      intros H H'. early "HA HB".
+      iApply mwp_value'. iApply "HB". rewrite H'. iFrame. iApply H.
+    Qed.
+
+    Lemma run_spec {X} : forall (e : mon X) (Φ : X -> iProp Σ) (p : state * X) (s : state),
+        run e s = Res p ->
+    |{{ True }}| e |{{ v, RET v; Φ v }}| -> Φ p.2.
+    Proof.
+      fix e 1.
+      destruct e0; intros.
+      - apply ret_spec_bis in H0. inversion H. apply H0.
+      - destruct s.
+        + inversion H.
+        + simpl in H. pose (e _ Φ _ _ H). apply u. simpl in H0. pose (heapG Σ). Print heapG.
+          pose (heapG_gen_heapG (heapG Σ)).
+          
+          Print gFunctors. Print rFunctor. Print heapG.
+          
+          
+          applye in H.
+          unfold mwp in H0. iApply H0. simpl in H0. iApply H0.
+    Qed.        
+  End proofmode_divers.
+  
+End proofmode.
 
 
 (* (* %%%%%%%%%%%%%%%%%%%%%%%%%%%%%%%%%%%%%%%%%Old%%%%%%%%%%%%%%%%%%% *) *)
@@ -274,17 +771,17 @@ End weakestpre_gensym.
 (* Module gensym. *)
 (*   Import monad. *)
 (*   Open Scope positive_scope. *)
-  
+
 (*   Definition ident := positive. *)
 (*   Definition state := gmap ident type. *)
-  
+
 (*   Inductive FreshMonad (X : Type) : Type := *)
 (*   | ret : X -> FreshMonad X *)
 (*   | Gensym: (ident -> FreshMonad X) -> FreshMonad X. *)
-  
+
 (*   Arguments ret {_} x. *)
 (*   Arguments Gensym {_} f. *)
-  
+
 (*   Fixpoint bind {X Y} (m: FreshMonad X) (k: X -> FreshMonad Y) : FreshMonad Y := *)
 (*     match m with *)
 (*     | ret x => k x *)
@@ -292,7 +789,7 @@ End weakestpre_gensym.
 (*     end. *)
 
 (*   Definition gensym := Gensym ret. *)
-  
+
 (*   Definition fresh (s : state) := map_fold (fun x _ res => Pos.max res (x+1)) 1 s. *)
 
 (*   Fixpoint run {X} (m : FreshMonad X) : state -> state * X := *)
@@ -320,7 +817,7 @@ End weakestpre_gensym.
 (*   Proof. split; eauto. Qed. *)
 
 (*   Canonical Structure gensym_monad := @Monad FreshMonad (gmap ident type) (@ret) (@bind) (@run) mP. *)
-  
+
 (* End gensym. *)
 
 
@@ -328,20 +825,20 @@ End weakestpre_gensym.
 (*   Export weakestpre. *)
 (*   Export gensym. *)
 (*   Export gen_heap. *)
-   
+
 (*   Class irisG (Σ : gFunctors) := *)
 (*     IrisG { *)
 (*         iris_invG :> invG.invG Σ; *)
 (*         state_interp : state → iProp Σ; *)
 (*       }. *)
 (*   Global Opaque iris_invG. *)
-  
+
 (*   Class heapG Σ := *)
 (*     HeapG { *)
 (*         heapG_invG : invG.invG Σ; *)
 (*         heapG_gen_heapG :> gen_heapG positive type Σ; *)
 (*       }. *)
-  
+
 (*   Instance heapG_irisG `{!heapG Σ} : irisG Σ := { *)
 (*                                                  iris_invG := heapG_invG; *)
 (*                                                  state_interp σ := gen_heap_ctx σ%I; *)
@@ -359,7 +856,7 @@ End weakestpre_gensym.
 (*     Implicit Types Φ : X → iProp Σ. *)
 (*     Implicit Types v : X. *)
 (*     Implicit Types e : FreshMonad X. *)
-    
+
 (*     Fixpoint mwp `{!irisG Σ} (e1 : FreshMonad X) (Q : X -> iProp Σ) : iProp Σ := *)
 (*       match e1 with *)
 (*       | ret v => Q v *)
@@ -420,3 +917,4 @@ End weakestpre_gensym.
   
 
 (* End weakestpre_gensym. *)
+
